GenRealSN.v
@@ -6,11 +6,12 @@ Require Import Models.
 
 Module Lc := Lambda.
 
-(* The abstract normalization model. *)
+(** * Abstract strong mormalization model (supporting strong eliminations) *)
 
 Module Type RealSN_addon (M : CC_Model).
   Import M.
 
+  (** Types are equipped with a saturated set *)
   Parameter Real : X -> X -> SAT.
   Parameter Real_morph: Proper (eqX ==> eqX ==> eqSAT) Real.
 
@@ -27,8 +28,7 @@ Module Type RealSN_addon (M : CC_Model).
 
   Existing Instance Real_morph.
 
-(* No empty types (False is inhabited) *)
-
+  (** Every proposition is inhabited *)
   Parameter daimon : X.
   Parameter daimon_false : daimon ∈ prod props (fun P => P).
 
@@ -43,11 +43,30 @@ Import MM.
 
 (* Derived properties of the abstract SN model *)
 
-(* We first introduce the realizability relation, which the conjunction
+(** We first introduce the realizability relation, which the conjunction
    of the value and term interpretation requirements.
    [x,t] \real T reads "t is a realizer of x as a value of type T".
  *)
 Notation "[ x , t ] \real A" := (x ∈ A  /\ inSAT t (Real A x)) (at level 60).
+
+Lemma real_daimon : forall x t T,
+  [x,t] \real T -> [x,SatSet.daimon] \real T.
+destruct 1; split; trivial.
+apply varSAT.
+Qed.
+
+Lemma real_sn : forall x A t, [x,t] \real A -> Lc.sn t.
+destruct 1 as (_,?).
+apply sat_sn in H; trivial.
+Qed.
+
+Lemma real_exp_K : forall x A u v,
+  Lc.sn v ->
+  [x,u] \real A ->
+  [x,Lc.App2 Lc.K u v] \real A. 
+destruct 2; split; trivial.
+apply KSAT_intro; trivial.
+Qed.
 
 Lemma piSAT_intro : forall A B f t,
   Lc.sn t -> (* if A is empty *)
@@ -104,10 +123,9 @@ apply prod_intro_sn; intros; trivial.
 
  destruct H2 with (1:=H3).
  split; trivial.
+ apply inSAT_exp; trivial.
  destruct H3.
- apply prodSAT_elim with (Real dom x); trivial.
- apply prodSAT_intro; intros.
- apply H2; auto.
+ apply sat_sn in H6; auto.
 Qed.
 
 Lemma prod_elim : forall dom f x F t u,
@@ -125,167 +143,24 @@ split.
 Qed.
 
 
-Lemma real_sn : forall x A t, [x,t] \real A -> Lc.sn t.
-destruct 1 as (_,?).
-apply sat_sn in H; trivial.
-Qed.
 
-Lemma real_exp_K : forall x A u v,
-  Lc.sn v ->
-  [x,u] \real A ->
-  [x,Lc.App2 Lc.K u v] \real A. 
-destruct 2; split; trivial.
-apply KSAT_intro; trivial.
-Qed.
-
-
-(* Now the abstract strong normalization proof. *)
+(** The abstract strong normalization proof. *)
 Require ObjectSN.
 Include ObjectSN.MakeObject(M).
 
 
-(* Dealing with top sorts.
-   We prove all types of top sorts are inhabited. *)
+(** * Semantic typing relation. *)
 
-Fixpoint cst_fun (i:val) (e:list trm) (x:X) : X :=
-  match e with
-  | List.nil => x
-  | T::f => lam (int i T) (fun y => cst_fun (V.cons y i) f x)
-  end.
-
-Instance cst_morph : Proper (eq_val ==> @eq _ ==> eqX ==> eqX) cst_fun.
-do 4 red; intros.
-subst y0.
-revert x y H.
-induction x0; simpl; intros; auto.
-apply lam_ext; intros.
- rewrite H; reflexivity.
-
- red; intros.
- apply IHx0.
- rewrite H2; rewrite H; reflexivity.
-Qed.
-
-Fixpoint cst_trm (e:list trm) (x:Lc.term) : Lc.term :=
-  match e with
-  | List.nil => x
-  | T::f => Lc.Abs (Lc.lift 1 (cst_trm f x))
-  end.
-
-
-Lemma cst_trm_sn : forall e t,
-  Lc.sn t -> Lc.sn (cst_trm e t).
-induction e; simpl; intros; auto.
-apply Lc.sn_abs.
-apply Lc.sn_lift; auto.
-Qed.
-
-Lemma wit_prod : forall x U t,
-  (forall i, [x,t] \real int i U) ->
-  forall e i,
-  [cst_fun i e x, cst_trm e t] \real int i (prod_list e U).
-induction e; simpl; intros; auto.
-apply prod_intro_lam; intros; auto.
- red; intros.
- rewrite H1; reflexivity.
-
- red; intros.
- rewrite H1; reflexivity.
-
- apply Lc.sn_lift.
- apply cst_trm_sn.
- apply real_sn with x (int i U); auto.
-
- unfold Lc.subst; rewrite Lc.simpl_subst; auto with arith.
- rewrite Lc.lift0.
- trivial.
-Qed.
-
-
-(* We could parameterize non_empty with a val [i0], and
-   quantify over i s.t. vshift (length e) i = i0.
-   This would allow kind variables. *)
-Definition non_empty T :=
-  exists e, exists2 U, eq_trm T (prod_list e U) &
-    exists x t, forall i, [x,t] \real int i U.
-
-Instance non_empty_morph : Proper (eq_trm ==> iff) non_empty.
-unfold non_empty; do 2 red; intros.
-split; intros (e,(U,eq_U,inU)); exists e;
-  exists U; trivial.
- rewrite <- H; trivial.
- rewrite H; trivial.
-Qed.
-
-Lemma prop_non_empty : non_empty prop.
-exists List.nil; exists prop; simpl prod_list.
- reflexivity.
-
- exists (prod props (fun P => P)); exists Lc.K; intro i.
- assert (prod props (fun P => P) ∈ props).
-  apply impredicative_prod; intros; auto.
-  red; auto.
- split; trivial.
- simpl; rewrite Real_sort; trivial.
- apply Lc.sn_K.
-Qed.
-
-Lemma prod_non_empty : forall T U,
-  non_empty U ->
-  non_empty (Prod T U).
-intros.
-destruct H as (e,(U',eq_U,wit_U)).
-exists (T::e); exists U'; simpl prod_list; trivial.
-rewrite eq_U; reflexivity.
-Qed.
-
-Lemma non_empty_witness : forall i T,
-  non_empty T ->
-  exists x, exists u, [x,u] \real int i T.
-intros.
-destruct H as (e,(U,eq_U,(wit1,(wit2,in_U)))).
-exists (cst_fun i e wit1); exists (cst_trm e wit2).
-rewrite eq_U.
-apply wit_prod; trivial.
-Qed.
-
-Lemma non_empty_lift M k :
-  non_empty M <-> non_empty (lift_rec 1 k M).
-unfold non_empty; split; intros.
- destruct H as (e,(U,?,(x,(t,?)))).
- destruct lift_prod_list_ex with 1 k e U as (e',?).
- exists e'.
- exists (lift_rec 1 (length e+k) U).
-  rewrite H; trivial.
-
-  exists x; exists t; intros.
-  rewrite int_lift_rec_eq.
-  apply H0.
-
- destruct H as (e,(U,?,(x,(t,?)))).
- destruct subst_prod_list_ex with (Ref 0) k e U as (e',?).
- exists e'.
- exists (subst_rec (Ref 0) (length e+k) U).
-  rewrite <- H1.
-  rewrite <- H.
-  apply simpl_subst_lift_rec.
-
-  exists x; exists t; intros.
-  rewrite int_subst_rec_eq.
-  apply H0.
-Qed.
-
-(* Semantic typing relation.
-   Handles the case of kind: a type that contains all "non-empty" types
-   and that is included in no type.
+(** Handles the case of kind: a type that contains all "non-empty" types
+    and that is included in no type.
  *)
 
 Definition in_int (i:val) (j:Lc.intt) (M T:trm) :=
   M <> None /\
   match T with
-  (* M has type kind *)
-  | None => non_empty M /\ Lc.sn (tm j M)
-  (* T is a regular type *)
+  (** M has type kind *)
+  | None => kind_ok M /\ Lc.sn (tm j M)
+  (** T is a regular type *)
   | _ => [int i M, tm j M] \real int i T
   end.
 
@@ -346,7 +221,7 @@ split; try discriminate.
   rewrite int_cons_lift_eq; trivial.
 
   destruct mem; split; trivial.
-  rewrite non_empty_lift with (k:=0) in H.
+  rewrite kind_ok_lift with (k:=0) in H.
   rewrite eq_trm_lift_ref_fv in H; auto with arith.
 Qed.
 
@@ -359,7 +234,7 @@ destruct T; simpl in mem.
  destruct mem; trivial.
 Qed.
 
-(* Environments *)
+(** Environments *)
 Definition env := list trm.
 
 Definition val_ok (e:env) (i:val) (j:Lc.intt) :=
@@ -403,7 +278,9 @@ apply varSAT.
 Qed.
 
 
-(* Judgements *)
+(** * Judgements *)
+
+(** #<a name="MakeModel.wf"></a># *)
 Definition wf (e:env) :=
   exists i, exists j, val_ok e i j.
 Definition typ (e:env) (M T:trm) :=
@@ -458,7 +335,7 @@ destruct T; try contradiction.
 apply H0; trivial.
 Qed.
 
-
+(** Well-formed types *)
 Definition typs e T :=
   typ e T kind \/ typ e T prop.
 
@@ -471,15 +348,19 @@ Qed.
 Lemma typs_non_empty : forall e T i j,
   typs e T ->
   val_ok e i j ->
-  exists x, exists u, [x,u] \real int i T.
+  exists x, [x,SatSet.daimon] \real int i T.
 intros.
 destruct H.
  apply H in H0.
- destruct H0 as (_,(mem,_)); apply non_empty_witness; trivial.
+ destruct H0 as (_,(mem,_)).
+ destruct kind_ok_witness with (1:=mem) (i:=i) as (w,?); exists w.
+ split; trivial.
+ apply varSAT.
 
  apply H in H0.
  destruct H0 as (_,mem); simpl in *.
- exists (app daimon (int i T)); exists (Lc.App SatSet.daimon (tm j T)).
+ exists (app daimon (int i T)).
+ apply real_daimon with (Lc.App SatSet.daimon (tm j T)).
  apply prod_elim with (dom:=props) (F:=fun P => P); trivial.
   red; intros; trivial.
 
@@ -487,7 +368,7 @@ destruct H.
 Qed.
 
 
-(* Strong normalization *)
+(** * Strong normalization *)
 
 Lemma typs_sn : forall e T i j, typs e T -> val_ok e i j -> Lc.sn (tm j T).
 destruct 1 as [ty_T|ty_T]; intro is_val; apply ty_T in is_val;
@@ -496,9 +377,9 @@ destruct 1 as [ty_T|ty_T]; intro is_val; apply ty_T in is_val;
  destruct is_val as (_,mem); apply real_sn in mem; trivial.
 Qed.
 
-(* This lemma shows that the abstract model construction entails
+(** This lemma shows that the abstract model construction entails
    strong normalization.
-   At this level, we do have the actual syntax. However, red_term
+   At this level, we do not have the actual syntax. However, red_term
    is a relation on the denotations that admits the same introduction
    rules as the syntactic reduction.
    When the syntax is introduced, it will only remain to check that
@@ -515,7 +396,10 @@ apply in_int_sn in is_val.
 apply simul with (1:=is_val) (2:=eq_refl).
 Qed.
 
-(* Context formation rules *)
+
+(** * Inference rules *)
+
+(** ** Context formation rules *)
 
 Lemma wf_nil : wf List.nil.
 red.
@@ -532,12 +416,12 @@ unfold wf; intros.
 assert (T <> kind).
  apply typs_not_kind in H0; trivial.
 destruct H as (i,(j,is_val)).
-destruct typs_non_empty with (1:=H0) (2:=is_val) as (x,(u,non_mt)).
-exists (V.cons x i); exists (I.cons u j).
+destruct typs_non_empty with (1:=H0) (2:=is_val) as (x,non_mt).
+exists (V.cons x i); exists (I.cons SatSet.daimon j).
 apply vcons_add_var; trivial.
 Qed.
 
-(* Extensional equality rules *)
+(** ** Extensional equality rules *)
 
 Lemma refl : forall e M, eq_typ e M M.
 red; simpl; reflexivity.
@@ -618,7 +502,7 @@ rewrite beta_eq.
  destruct real_arg; trivial.
 Qed.
 
-(* Intensional equality *)
+(** ** Intensional equality *)
 
 Instance eq_typ'_equiv : forall e, Equivalence (eq_typ' e).
 split; red; intros.
@@ -679,13 +563,13 @@ destruct 1; destruct 1; split.
  apply conv_term_beta; trivial.
 Qed.
 
-(* Typing rules *)
+(** ** Typing rules *)
 
 Lemma typ_prop : forall e, typ e prop kind.
 red; simpl; intros.
 split; try discriminate.
 split; simpl; auto.
- apply prop_non_empty.
+ apply prop_kind_ok.
 
  apply Lc.sn_K.
 Qed.
@@ -722,7 +606,7 @@ Lemma prod_intro2 : forall dom f F t m,
   eq_fun dom f f ->
   eq_fun dom F F ->
   Lc.sn t ->
-  (exists x, exists u, [x,u] \real dom) ->
+  (exists x, [x,SatSet.daimon] \real dom) ->
   (forall x u, [x, u] \real dom -> [f x, Lc.subst u m] \real F x) ->
   [lam dom f, CAbs t m] \real prod dom F.
 intros.
@@ -730,10 +614,9 @@ apply prod_intro_lam in H3; trivial.
 unfold CAbs; apply real_exp_K; trivial.
 (* *)
 destruct H2.
-destruct H2.
 apply H3 in H2.
 apply real_sn in H2.
-apply Lc.sn_subst with x0; trivial.
+apply Lc.sn_subst in H2; trivial.
 Qed.
 
 Lemma typ_abs : forall e T M U,
@@ -762,19 +645,6 @@ apply prod_intro2; intros.
  rewrite <- tm_subst_cons; trivial.
 Qed.
 
-Lemma typ_beta : forall e T M N U,
-  typs e T ->
-  typ (T::e) M U ->
-  typ e N T ->
-  T <> kind ->
-  U <> kind ->
-  typ e (App (Abs T M) N) (subst N U).
-Proof.
-intros.
-apply typ_app with T; trivial.
-apply typ_abs; trivial.
-Qed.
-
 Lemma typ_prod : forall e T U s2,
   s2 = kind \/ s2 = prop ->
   typs e T ->
@@ -786,13 +656,13 @@ assert (T_not_tops : T <> kind).
  destruct ty_T as [ty_T|ty_T]; apply ty_T in is_val;
    destruct is_val; trivial.
 assert (typs (T::e) U) by (destruct is_srt; subst; red; auto).
-destruct (typs_non_empty ty_T is_val) as (witT,(witt,in_T)).
+destruct (typs_non_empty ty_T is_val) as (witT,in_T).
 specialize vcons_add_var with (1:=is_val) (2:=in_T) (3:=T_not_tops);
   intros in_U.
 apply ty_U in in_U.
 split;[discriminate|simpl].
 assert (snU : Lc.sn (tm (Lc.ilift j) U)).
- apply Lc.sn_subst with witt.
+ apply Lc.sn_subst with SatSet.daimon.
  rewrite <- tm_subst_cons.
  destruct is_srt; subst s2; simpl in *.
   destruct in_U as (_,(_,snu)); trivial.
@@ -802,7 +672,7 @@ assert (snU : Lc.sn (tm (Lc.ilift j) U)).
 destruct is_srt; subst s2; simpl in *.
  (* s2=kind *)
  split.
-  apply prod_non_empty.
+  apply prod_kind_ok.
   destruct in_U as (_,(mem,_)); trivial.
 
   apply Lc.sn_K2.
@@ -845,7 +715,7 @@ apply in_int_intro; trivial.
 rewrite <- H0; trivial.
 Qed.
 
-(* Weakening *)
+(** Weakening *)
 
 Lemma weakening : forall e M T A,
   typ e M T ->
@@ -862,7 +732,7 @@ assert (val_ok e (V.lams 0 (V.shift 1) i) (I.lams 0 (I.shift 1) j)).
 
   intros (_,(ne,sat)); split;[discriminate|split; trivial].
 
-  rewrite non_empty_lift with (k:=0).
+  rewrite kind_ok_lift with (k:=0).
   rewrite eq_trm_lift_ref_fv; auto with *.
 destruct H with (1:=H1) as (M_nk, inT).
 split.
@@ -874,13 +744,13 @@ split.
  rewrite tm_lift_rec_eq; trivial.
 
  destruct inT; split.
-  unfold lift; rewrite <- non_empty_lift; trivial.
+  unfold lift; rewrite <- kind_ok_lift; trivial.
 
   unfold lift; rewrite tm_lift_rec_eq; trivial.
 Qed.
 
 
-(* Subtyping rules *)
+(** ** Subtyping rules *)
 
 Lemma sub_refl : forall e M M',
   eq_typ e M M' -> sub_typ e M M'.
@@ -918,7 +788,7 @@ apply in_int_not_kind in H; trivial.
 apply in_int_intro; auto.
 Qed.
 
-(* Covariance can be derived if we have a weak eta property:
+(** Covariance can be derived if we have a weak eta property:
    any function is a lambda abstraction *with the same domain*.
    This is OK with set-theoretical functions (in contrast with
    general eta which does not hold on set-theoretical functions).
